WIP

NuInstructions.thy
@@ -121,30 +121,37 @@ lemma [simp]: "(if P then a \<R_arr_tail> x else a \<R_arr_tail> x') = a \<R_arr
 
 subsubsection \<open>Stack Head\<close> \<comment> \<open>A technically auxiliary \<nu>-abstractor\<close>
 
-definition Nu_Stack_Head :: "('a::lrep,'ax) \<nu> \<Rightarrow> (heap \<times> 'stack,'hsx) \<nu> \<Rightarrow> (heap \<times> 'a \<times> 'stack, 'ax \<times> 'hsx) \<nu>"
-  where "Nu_Stack_Head A Ctx = (\<lambda>(ax,hsx). {(h,a,s). (a \<nuLinkL> A \<nuLinkR> ax) \<and> ((h,s) \<nuLinkL> Ctx \<nuLinkR> (hsx))} )"
+definition Nu_Front_Stack :: "('a::lrep,'ax) \<nu> \<Rightarrow> (heap \<times> 'stack,'hsx) \<nu> \<Rightarrow> (heap \<times> 'a \<times> 'stack, 'ax \<times> 'hsx) \<nu>"
+  where "Nu_Front_Stack A Ctx = (\<lambda>(ax,hsx). {(h,a,s). (a \<nuLinkL> A \<nuLinkR> ax) \<and> ((h,s) \<nuLinkL> Ctx \<nuLinkR> (hsx))} )"
 
-consts "Stack_Head_sugar" :: " 'just \<Rightarrow> 'a \<Rightarrow> 'sugar " ( "_/ <stack-head> _" [13,14] 13) \<comment> \<open>Note it is left associative\<close>
-translations " c \<tycolon> Ctx <stack-head> a \<tycolon> A " == " (CONST Pair a c) \<tycolon> (CONST Nu_Stack_Head A Ctx) "
-  " Ctx <stack-head> A " => " (CONST Pair (_\<nu>typing_x A) (_\<nu>typing_x Ctx)) \<tycolon> (CONST Nu_Stack_Head (_\<nu>typing_ty A) (_\<nu>typing_ty Ctx)) "
+consts "Front_Stack_sugar" :: " 'just \<Rightarrow> 'a \<Rightarrow> 'sugar " ( "_/ \<heavy_comma>^ _" [13,14] 13) \<comment> \<open>Note it is left associative\<close>
+translations " c \<tycolon> Ctx \<heavy_comma>^ a \<tycolon> A " == " (CONST Pair a c) \<tycolon> (CONST Nu_Front_Stack A Ctx) "
+  " Ctx \<heavy_comma>^ A " => " (CONST Pair (_\<nu>typing_x A) (_\<nu>typing_x Ctx)) \<tycolon> (CONST Nu_Front_Stack (_\<nu>typing_ty A) (_\<nu>typing_ty Ctx)) "
 
-lemma [simp]: "(h,a,s) \<nuLinkL> Nu_Stack_Head A Ctx \<nuLinkR> (ax,hsx) \<longleftrightarrow> (a \<nuLinkL> A \<nuLinkR> ax) \<and> ((h,s) \<nuLinkL> Ctx \<nuLinkR> hsx)"
-  unfolding Nu_Stack_Head_def Refining_def by simp
-lemma [simp]: "\<tort_lbrace> (a,h,s) \<tycolon> Nu_Stack_Head A (NuTopCtx H S) \<tort_rbrace> = \<tort_lbrace> (h,a,s) \<tycolon> NuTopCtx H (A <stack-div> S) \<tort_rbrace>" by auto
-lemma [simp]: "\<tort_lbrace>c \<tycolon> Ctx \<and>\<^sup>\<nu>\<^sub>a\<^sub>u\<^sub>t\<^sub>o P <stack-head> x \<tycolon> T\<tort_rbrace> = \<tort_lbrace> (c \<tycolon> Ctx <stack-head> x \<tycolon> T) \<and>\<^sup>\<nu>\<^sub>a\<^sub>u\<^sub>t\<^sub>o P \<tort_rbrace>" unfolding Auto_def by auto
+text \<open>Normally the stack elements are written `before` the heap elements, \<^term>\<open>s1 \<tycolon> S1\<heavy_comma> s2 \<tycolon> S2\<heavy_comma> \<^bold>h\<^bold>e\<^bold>a\<^bold>p h \<tycolon> H\<close>.
+  The \<^term>\<open>Nu_Front_Stack\<close> allows one writes the stack elements `after` the heap, as \<^term>\<open>s1 \<tycolon> S1\<heavy_comma> \<^bold>h\<^bold>e\<^bold>a\<^bold>p h \<tycolon> H \<heavy_comma>^ s2 \<tycolon> S2\<close>.
+  Both of the two \<nu>-types specify the same low concretes.
+  It is useful when one needs to specify over the whole remaining stack and heap, e.g., theorem `Until` (see later)
+    which requires body to return \<^term>\<open>x \<tycolon> X \<heavy_comma>^ loop_condition \<tycolon> \<bool>\<close> where the \<^term>\<open>x \<tycolon> X\<close> instantiated by caller
+    specifies all the heap and remaining stack except the leading loop_condition.\<close>
 
-lemma Nu_Stack_Head_cong: "\<tort_lbrace>c \<tycolon> Ctx\<tort_rbrace> \<equiv> \<tort_lbrace>c' \<tycolon> Ctx'\<tort_rbrace> \<Longrightarrow> \<tort_lbrace>c \<tycolon> Ctx <stack-head> x \<tycolon> T\<tort_rbrace> \<equiv> \<tort_lbrace>c' \<tycolon> Ctx' <stack-head> x \<tycolon> T\<tort_rbrace>"
+lemma [simp]: "(h,a,s) \<nuLinkL> Nu_Front_Stack A Ctx \<nuLinkR> (ax,hsx) \<longleftrightarrow> (a \<nuLinkL> A \<nuLinkR> ax) \<and> ((h,s) \<nuLinkL> Ctx \<nuLinkR> hsx)"
+  unfolding Nu_Front_Stack_def Refining_def by simp
+lemma [simp]: "\<tort_lbrace> (a,h,s) \<tycolon> Nu_Front_Stack A (NuTopCtx H S) \<tort_rbrace> = \<tort_lbrace> (h,a,s) \<tycolon> NuTopCtx H (A <stack-div> S) \<tort_rbrace>" by auto
+lemma [simp]: "\<tort_lbrace>c \<tycolon> Ctx \<and>\<^sup>\<nu>\<^sub>a\<^sub>u\<^sub>t\<^sub>o P \<heavy_comma>^ x \<tycolon> T\<tort_rbrace> = \<tort_lbrace> (c \<tycolon> Ctx \<heavy_comma>^ x \<tycolon> T) \<and>\<^sup>\<nu>\<^sub>a\<^sub>u\<^sub>t\<^sub>o P \<tort_rbrace>" unfolding Auto_def by auto
+
+lemma Nu_Front_Stack_cong: "\<tort_lbrace>c \<tycolon> Ctx\<tort_rbrace> \<equiv> \<tort_lbrace>c' \<tycolon> Ctx'\<tort_rbrace> \<Longrightarrow> \<tort_lbrace>c \<tycolon> Ctx \<heavy_comma>^ x \<tycolon> T\<tort_rbrace> \<equiv> \<tort_lbrace>c' \<tycolon> Ctx' \<heavy_comma>^ x \<tycolon> T\<tort_rbrace>"
   unfolding atomize_eq by auto
-simproc_setup Nu_Stack_Head_cong ("\<tort_lbrace>c \<tycolon> Ctx <stack-head> x \<tycolon> T\<tort_rbrace>") = \<open>K (NuSimpCong.simproc @{thm Nu_Stack_Head_cong})\<close>
+simproc_setup Nu_Front_Stack_cong ("\<tort_lbrace>c \<tycolon> Ctx \<heavy_comma>^ x \<tycolon> T\<tort_rbrace>") = \<open>K (NuSimpCong.simproc @{thm Nu_Front_Stack_cong})\<close>
 
-lemma [\<nu>intro]: "\<^bold>c\<^bold>a\<^bold>s\<^bold>t R\<heavy_comma> \<^bold>h\<^bold>e\<^bold>a\<^bold>p H \<longmapsto> c \<tycolon> Ctx \<^bold>w\<^bold>i\<^bold>t\<^bold>h P \<^bold>w\<^bold>h\<^bold>e\<^bold>n Q \<Longrightarrow> \<^bold>i\<^bold>n\<^bold>t\<^bold>r\<^bold>o \<^bold>c\<^bold>a\<^bold>s\<^bold>t R\<heavy_comma> x \<tycolon> X\<heavy_comma> \<^bold>h\<^bold>e\<^bold>a\<^bold>p H \<longmapsto> c \<tycolon> Ctx <stack-head> (x \<tycolon> X) \<^bold>w\<^bold>h\<^bold>e\<^bold>n Q"
+lemma [\<nu>intro]: "\<^bold>c\<^bold>a\<^bold>s\<^bold>t R\<heavy_comma> \<^bold>h\<^bold>e\<^bold>a\<^bold>p H \<longmapsto> c \<tycolon> Ctx \<^bold>w\<^bold>i\<^bold>t\<^bold>h P \<^bold>w\<^bold>h\<^bold>e\<^bold>n Q \<Longrightarrow> \<^bold>i\<^bold>n\<^bold>t\<^bold>r\<^bold>o \<^bold>c\<^bold>a\<^bold>s\<^bold>t R\<heavy_comma> x \<tycolon> X\<heavy_comma> \<^bold>h\<^bold>e\<^bold>a\<^bold>p H \<longmapsto> c \<tycolon> Ctx \<heavy_comma>^ (x \<tycolon> X) \<^bold>w\<^bold>h\<^bold>e\<^bold>n Q"
   unfolding Intro_def Cast_def by simp
 lemma [\<nu>intro]: "\<^bold>c\<^bold>a\<^bold>s\<^bold>t c \<tycolon> Ctx \<longmapsto> (R\<heavy_comma> \<^bold>h\<^bold>e\<^bold>a\<^bold>p H) \<^bold>w\<^bold>i\<^bold>t\<^bold>h P \<^bold>w\<^bold>h\<^bold>e\<^bold>n Q \<Longrightarrow> \<^bold>p\<^bold>r\<^bold>e\<^bold>m\<^bold>i\<^bold>s\<^bold>e Q
-    \<Longrightarrow> \<^bold>d\<^bold>e\<^bold>s\<^bold>t \<^bold>c\<^bold>a\<^bold>s\<^bold>t c \<tycolon> Ctx <stack-head> (x \<tycolon> X) \<longmapsto> (R\<heavy_comma> x \<tycolon> X\<heavy_comma> \<^bold>h\<^bold>e\<^bold>a\<^bold>p H) \<^bold>w\<^bold>i\<^bold>t\<^bold>h P"
+    \<Longrightarrow> \<^bold>d\<^bold>e\<^bold>s\<^bold>t \<^bold>c\<^bold>a\<^bold>s\<^bold>t c \<tycolon> Ctx \<heavy_comma>^ (x \<tycolon> X) \<longmapsto> (R\<heavy_comma> x \<tycolon> X\<heavy_comma> \<^bold>h\<^bold>e\<^bold>a\<^bold>p H) \<^bold>w\<^bold>i\<^bold>t\<^bold>h P"
   unfolding Dest_def Cast_def by simp blast
 
 
-  subsubsection \<open>until\<close>
+subsubsection \<open>until\<close>
 
 inductive SemUnt :: "('r \<longmapsto> 1 word \<times> 'r) \<Rightarrow> heap \<times> 'r \<Rightarrow> 'r state \<Rightarrow> bool" where
   "f s = Success (h,0,r) \<Longrightarrow> SemUnt f s (Success (h,r))"
@@ -169,7 +176,7 @@ definition Until :: "('r \<longmapsto> 1 word \<times> 'r) \<Rightarrow> 'r \<lo
   "Until f s = (if (\<exists>y. SemUnt f s y) then The (SemUnt f s) else PartialCorrect)"
 
 
-lemma Until: "(\<forall>x. \<^bold>p\<^bold>r\<^bold>o\<^bold>c body \<blangle> x \<tycolon> X \<longmapsto> \<exists>* x'. x' \<tycolon> X <stack-head> c x' \<tycolon> \<bool> \<brangle>)
+lemma "__Until___\<nu>proc": "(\<forall>x. \<^bold>p\<^bold>r\<^bold>o\<^bold>c body \<blangle> x \<tycolon> X \<longmapsto> \<exists>* x'. x' \<tycolon> X \<heavy_comma>^ c x' \<tycolon> \<bool> \<brangle>)
   \<longrightarrow> \<^bold>p\<^bold>r\<^bold>o\<^bold>c Until body \<blangle> x \<tycolon> X \<longmapsto> \<exists>*x'. x' \<tycolon> X \<and>\<^sup>\<nu>' (\<not> c x') \<brangle>"
   for X :: "(heap \<times> 'a::lrep, 'b) \<nu>"
   unfolding Until_def Procedure_def Auto_def
@@ -189,14 +196,16 @@ let open Parse Scan NuHelp NuBasics in
   $$$ "until" |-- vars -- option ($$$ "in" |-- list1 term)
      -- option ($$$ "heap" |-- list1 term) -- ($$$ "subj" |-- term) -- Scan.option ($$$ "always" |-- term)
     >> (fn ((((vars, stack_schema), heap_schema), subj), always) => fn _ =>
-      NuLoop.mk_loop_proc @{thm Until} vars stack_schema heap_schema subj always ctx meta)
+      NuLoop.mk_loop_proc @{thm "__Until___\<nu>proc"} vars stack_schema heap_schema subj always ctx meta)
 end\<close>
 
+subsubsection \<open>while\<close>
 
-notepad
-begin
-  assume A[simplified Auto_def]: "\<^bold>p\<^bold>r\<^bold>o\<^bold>c f \<blangle>  x \<tycolon> Auto NuRefine T P \<longmapsto> Y \<brangle>"
-end
+
+proc "while": \<open>x \<tycolon> X\<close> \<longmapsto> \<open>x \<tycolon> X\<close>
+  requires Cond_\<nu>proc: "\<forall>x. \<^bold>p\<^bold>r\<^bold>o\<^bold>c Cond \<blangle> x \<tycolon> X \<longmapsto> \<exists>* x'. x' \<tycolon> X \<heavy_comma>^ c x \<tycolon> \<bool> \<brangle>"
+    and Body_\<nu>proc: "\<forall>x. \<^bold>p\<^bold>r\<^bold>o\<^bold>c Body \<blangle> x \<tycolon> X \<longmapsto> \<exists>* x'. x' \<tycolon> X' \<brangle>"
+  \<bullet> "__Until__" \<medium_left_bracket> \<bullet> Cond 
 
 (*
   term \<open>(\<lambda>c. c) \<tycolon> Named (NAME xx) (ExNu (\<lambda>c. T))\<close>
